theories/IPM.v
@@ -12,7 +12,7 @@ Set Typeclasses Depth 5.
 
 Create HintDb iprop.
 Ltac uipropall :=
-  try (autounfold with iprop; autorewrite with iprop;
+  repeat (autounfold with iprop; autorewrite with iprop;
        all_once_fast ltac:(fun H => autounfold with iprop in H; autorewrite with iprop in H); ss).
 
 Section IPROP.
@@ -436,13 +436,6 @@ Infix "**" := bi_sep (at level 99).
 Infix "-*" := bi_wand (at level 99, right associativity).
 Notation "#=> P" := ((@bupd (bi_car (@iProp _)) (@bi_bupd_bupd (@iProp _) (@iProp_bi_bupd _))) P) (at level 99).
 
-From iris.algebra Require Import proofmode_classes.
-From iris.proofmode Require Import classes.
-From iris.base_logic Require Export derived.
-From iris.prelude Require Import options.
-
-Import base_logic.bi.uPred.
-
 Class IsOp {A : URA.t} (a b1 b2 : A) := is_op : a = URA.add b1 b2.
 Global Arguments is_op {_} _ _ _ {_}.
 Global Hint Mode IsOp + - - - : typeclass_instances.
@@ -460,9 +453,8 @@ Global Hint Mode IsOp'LR + ! - - : typeclass_instances.
 Global Instance is_op_lr_op {A : URA.t} (a b : A) : IsOp'LR (URA.add a b) a b | 0.
 Proof. by rewrite /IsOp'LR /IsOp. Qed.
 
-#[export] Hint Unfold iProp bi_entails bi_sep bi_and bi_or bi_wand bupd bi_bupd_bupd: iprop.
+#[export] Hint Unfold bi_entails bi_sep bi_and bi_or bi_wand bupd bi_bupd_bupd: iprop.
 
-(* Setup of the proof mode *)
 Section class_instances.
   Context `{Σ: GRA.t}.
 
@@ -470,84 +462,18 @@ Section class_instances.
     :
       Own a ⊢ #=> P.
   Proof.
-    uipropall. ss. i. unfold URA.extends in *. des. subst. ss.
-
-
-    Set Printing All.
-
-  Global Instance from_sep_ownM (a b1 b2 : Σ) :
-    IsOp a b1 b2 →
-    FromSep (Own a) (Own b1) (Own b2).
-  Proof.
-    ii. inv H. red. uipropall. i. des. subst.
-    unfold URA.extends in *. des. subst.
-    exists (URA.add ctx0 ctx). repeat rewrite URA.add_assoc.
-    f_equal. rewrite URA.add_comm. rewrite URA.add_assoc. f_equal.
-    eapply URA.add_comm.
+    uipropall. ss. i. unfold URA.extends in *. des. subst.
+    uipropall. i. esplits; [|apply SAT]. eapply URA.wf_mon.
+    instantiate (1:=ctx0). replace (a ⋅ ctx ⋅ ctx0) with (a ⋅ ctx0 ⋅ ctx); et.
+    repeat rewrite <- URA.add_assoc. f_equal. eapply URA.add_comm.
   Qed.
 
-  Global Instance into_and_ownM p (a b1 b2 : Σ) :
-    IsOp a b1 b2 → IntoAnd p (Own a) (Own b1) (Own b2).
-  Proof.
-    ii. apply bi.intuitionistically_if_mono. inv H.
-    uipropall. i. unfold URA.extends in *. des. subst. split.
-    { exists (URA.add b2 ctx). eapply URA.add_assoc. }
-    { exists (URA.add b1 ctx). rewrite URA.add_assoc.
-      f_equal. eapply URA.add_comm. }
-  Qed.
-
-  Global Instance into_sep_ownM (a b1 b2 : Σ) :
-    IsOp a b1 b2 → IntoSep (Own a) (Own b1) (Own b2).
-  Proof.
-    ii. red. inv H. uipropall. i.
-    unfold URA.extends in *. des. subst.
-    exists b1, (URA.add b2 ctx). split.
-    { symmetry. eapply URA.add_assoc. }
-    esplits.
-    { eapply URA.unit_id. }
-    { et. }
-  Qed.
-End class_instances.
-
-
-From iris.algebra Require Import proofmode_classes.
-From iris.proofmode Require Import classes.
-From iris.base_logic Require Export derived.
-From iris.prelude Require Import options.
-
-Import base_logic.bi.uPred.
-
-Class IsOp {A : URA.t} (a b1 b2 : A) := is_op : a = URA.add b1 b2.
-Global Arguments is_op {_} _ _ _ {_}.
-Global Hint Mode IsOp + - - - : typeclass_instances.
-
-Global Instance is_op_op {A : URA.t} (a b : A) : IsOp (URA.add a b) a b | 100.
-Proof. by rewrite /IsOp. Qed.
-
-Class IsOp' {A : URA.t} (a b1 b2 : A) := is_op' :> IsOp a b1 b2.
-Global Hint Mode IsOp' + ! - - : typeclass_instances.
-Global Hint Mode IsOp' + - ! ! : typeclass_instances.
-
-Class IsOp'LR {A : URA.t} (a b1 b2 : A) := is_op_lr : IsOp a b1 b2.
-Existing Instance is_op_lr | 0.
-Global Hint Mode IsOp'LR + ! - - : typeclass_instances.
-Global Instance is_op_lr_op {A : URA.t} (a b : A) : IsOp'LR (URA.add a b) a b | 0.
-Proof. by rewrite /IsOp'LR /IsOp. Qed.
-
-#[export] Hint Unfold iProp bi_entails bi_sep bi_and bi_or bi_wand bupd bi_bupd_bupd: iprop.
-
-(* Setup of the proof mode *)
-Section class_instances.
-  Context `{Σ: GRA.t}.
-
-  Lemma from_semantic (a: Σ) (P: iProp') (SAT: P a)
+  Lemma to_semantic (a: Σ) (P: iProp') (SAT: Own a ⊢ P) (WF: URA.wf a)
     :
-      Own a ⊢ #=> P.
+      P a.
   Proof.
-    uipropall. ss. i. unfold URA.extends in *. des. subst. ss.
-
-
-    Set Printing All.
+    uipropall. eapply SAT; et. refl.
+  Qed.
 
   Global Instance from_sep_ownM (a b1 b2 : Σ) :
     IsOp a b1 b2 →
